{\tiny \begin{gather*}
	v^b = R_a^b v_a + t^b_{b\to a} 
	~
	{\tiny\scriptstyle \begin{pmatrix}
	v^b \\ 1
	\end{pmatrix}
	= \begin{pmatrix}
	R_a^b & t^b_{b\to a} \\
	0 & 1
	\end{pmatrix}
	\begin{pmatrix}
	v^a \\ 1
	\end{pmatrix}}
	\\
	T_2T_1 = \begin{pmatrix}
	R_2R_1 & R_2t_1+t_2 \\ 0 & 1
	\end{pmatrix}, ~ T^{-1} = \begin{pmatrix}
	R^T & -R^Tt \\ 0 & 1
	\end{pmatrix}\\
	{\tiny\scriptstyle R_a^b=\begin{pmatrix}
		 &  &  \\
		x_a^b & y_a^b & z_a^b \\
		 &  &  
		\end{pmatrix}=
	\begin{pmatrix}
	x_a\cdot x_b & y_a\cdot x_b & z_a\cdot x_b \\
	x_a\cdot y_b & y_a\cdot y_b & z_a\cdot y_b \\
	x_a\cdot z_b & y_a\cdot z_b & z_a\cdot z_b
	\end{pmatrix}}% 
	\\
	{\tiny {\scriptstyle R_x(\phi) R_y(\theta) R_z(\psi) }= 
	\begin{pmatrix}
		1 & 0 & 0 \\ 
		0 & c_\phi & -s_\phi \\
		0 & s_\phi & c_\phi 
	\end{pmatrix}~
	\begin{pmatrix}
		c_\theta & 0 & s_\theta \\ 
		0 & 1 & 0 \\
		-s_\theta & 0 & c_\theta
	\end{pmatrix}
	\begin{pmatrix}
		c_\psi & -s_\psi & 0 \\ 
		s_\psi & c_\psi & 0 \\
		0 & 0 & 1 
	\end{pmatrix}~
	} \\
	{\scriptstyle\tiny \text{convention: } x^G\doteq \left(R_C^G, t^G_{G\to 
	C}\right)} ~
	{\scriptstyle \text{re-projection error: }
	e = z_{observed}-\pi(x_{true}, l_{true})} \\
	{\tiny\scriptstyle \lambda \begin{pmatrix}
		u \\ v \\ 1
		\end{pmatrix} = 
	\begin{pmatrix}
	\tilde{u} \\ \tilde{v} \\ \tilde{w}
	\end{pmatrix} = K\underbrace{
	\left(\begin{array}{c|c}
	R_G^C & t^C_{C\to G}
	\end{array}\right)}_{M}
	\begin{pmatrix}
	x^G \\ y^G \\ z^G \\ 1
	\end{pmatrix} = 
	M\begin{pmatrix}
		x^G \\ y^G \\ z^G \\ 1
		\end{pmatrix}}, ~ {\tiny\scriptstyle K=\begin{pmatrix}
			\alpha_x & 0 & u_0 \\ 
			0 & \alpha_y & v_0 \\
			0 & 0 & 1
			\end{pmatrix}} \\ 
	{\scriptstyle\tiny u = \frac{m_{11}x + m_{12}y + m_{13}z + 
	m_{14}}{m_{31}x + m_{32}y + m_{33}z + m_{34}} \quad 
	v = \frac{m_{21}x + m_{22}y + m_{23}z + 
		m_{24}}{m_{31}x + m_{32}y + m_{33}z + m_{34}}} \\
	\text{\tiny $a_{x,y} = fk_{x,y}$, $u_0$, $v_0$ - PP in pixels}\hfill
\end{gather*}}